enable variable based benchmarking

experiments/coq-experiments/proplang/Analysis-SeedPool.py
@@ -59,10 +59,22 @@ def stacked_barchart_times(
     if not strategies:
         strategies = df.strategy.unique()
 
+    vmap = {
+        '0': 'HeapSeedPool',
+        '1': 'StaticSingletonPool',
+        '2': 'DynamicMonotonicSingletonPool',
+        '3': 'DynamicResettingSingletonPool',
+        '4': 'QueueSeedPool',
+    }
+
+    df['version'] = df['version'].apply(lambda x: vmap[x])
+
     versions = df.version.unique()
 
-    strategies = [f"{strategy[0]}-{strategy[1]}" for strategy in itertools.product(strategies, versions)]
+    print(versions)
 
+    strategies = [f"{strategy[0]}-{strategy[1]}" for strategy in itertools.product(strategies, versions)]
+    
     tasks = df.task.unique()
     total_tasks = len(tasks)
 
@@ -113,7 +125,7 @@ def stacked_barchart_times(
             title='',
             showticklabels=True,
         ),
-        font_size=60,
+        font_size=20,
         font={'family': 'Helvetica'},
         width=1920,
         height=1080,
@@ -188,10 +200,24 @@ def analyze(results: str, images: str):
         times = partial(stacked_barchart_times, case=workload, df=df)
         times(
             strategies=[
-                'BespokeFuzzer',
+                'TypeBasedFuzzer',
+                'BespokeFuzzer'
+            ],
+            # colors=['#000000', '#900D0D', '#DC5F00', '#243763', '#FFD700'],
+            limits=[0.1, 1, 10, 60],
+            limit_type='time',
+            image_path=images,
+            show=False,
+        )
+
+    for workload in ['STLCProplang', 'RBTProplang']:
+        times = partial(stacked_barchart_times, case=workload, df=df)
+        times(
+            strategies=[
+                'TypeBasedFuzzer',
             ],
             colors=['#000000', '#900D0D', '#DC5F00', '#243763', '#FFD700'],
-            limits=[0.001, 0.01, 0.1, 1],
+            limits=[0.1, 1, 10, 60],
             limit_type='time',
             image_path=images,
             show=False,
